ifc/extended/Testing/SanityChecks.v
@@ -36,10 +36,10 @@ Section Checkers.
                  (fun v => let '(Var lab st1 st2) := v in
                   property (indist lab st1 st2) : Gen QProp).
 
-  Definition prop_exec_preserves_well_formed (t : table) : Property Gen :=
+  Definition prop_fstep_preserves_well_formed (t : table) : Property Gen :=
     forAllShrink (* show *)(fun _ => ""%string) arbitrary (fun _ => []) (fun st =>
     (if well_formed st then
-      match exec t st with
+      match fstep t st with
       | Some (_, st') =>
 (*
         whenFail ("Initial: " ++ show st ++ nl ++
@@ -89,18 +89,18 @@ Lemma genState_well_formed : forall st,
   @genState Pred _ st <-> well_formed st.
 Admitted.
 
-Definition exec_preserves_well_formed t : Prop := forall st x st',
+Definition fstep_preserves_well_formed t : Prop := forall st x st',
   well_formed st ->
-  exec t st = Some (x, st') ->
+  fstep t st = Some (x, st') ->
   well_formed st'.
 
-Lemma prop_exec_preserves_well_formed_equiv :
+Lemma prop_fstep_preserves_well_formed_equiv :
   forall (t : table),
-    semProperty (@prop_exec_preserves_well_formed Pred _ t) <->
-    exec_preserves_well_formed t.
+    semProperty (@prop_fstep_preserves_well_formed Pred _ t) <->
+    fstep_preserves_well_formed t.
 Proof.
   move => t.
-  rewrite /prop_exec_preserves_well_formed /exec_preserves_well_formed
+  rewrite /prop_fstep_preserves_well_formed /fstep_preserves_well_formed
     semForAllShrink /arbitrary /arbState. setoid_rewrite semPredQProp.
   split => [H st tr st' wf ex | H st arb].
   - assert (@genState Pred _ st) as gs by (by rewrite genState_well_formed).
@@ -109,7 +109,7 @@ Proof.
     (* by move /semWhenFail_id /semBool in H. *)    
     by apply semBool in H.
   - move /genState_well_formed in arb. rewrite arb. specialize (H st).
-    move : H. case (exec t st) => [ [tr st'] | ] H.
+    move : H. case (fstep t st) => [ [tr st'] | ] H.
     + specialize (H tr st' arb Logic.eq_refl). rewrite H.
       (* rewrite semWhenFail_id. by rewrite <- semBool. *)
       by apply <- semBool.
